theories/interop/basics_resources.v
@@ -7,10 +7,14 @@ From melocoton Require Import named_props.
 From melocoton.ml_lang Require Import lang.
 From melocoton.interop Require Export basics.
 
-Class wrapperBasicsG `{SI: indexT} Σ := WrapperBasicsG {
+Class wrapperBasicsGpre `{SI: indexT} Σ := WrapperBasicsGpre {
   wrapperG_lstoreG :> ghost_mapG Σ lloc block;
   wrapperG_addr_lvalG :> ghost_mapG Σ addr lval;
   wrapperG_lloc_mapG :> ghost_mapG Σ lloc lloc_visibility;
+}.
+
+Class wrapperBasicsG `{SI: indexT} Σ := WrapperBasicsG {
+  wrapperG_inG :> wrapperBasicsGpre Σ;
   wrapperG_γζvirt : gname;
   wrapperG_γχvirt : gname;
   wrapperG_γroots_map : gname;
