theories/interop/gctoken.v
@@ -22,13 +22,17 @@ From melocoton.interop Require Import basics_resources.
    the wrapper WP and state interp.
  *)
 
-Class wrapperGCtokG `{SI: indexT} Σ := WrapperGCtokG {
-  wrapperG_basics :> wrapperBasicsG Σ;
+Class wrapperGCtokGpre `{SI: indexT} Σ := WrapperGCtokGpre {
   wrapperG_locsetG :> ghost_varG Σ (gsetUR loc);
   wrapperG_addrmapG :> ghost_varG Σ (leibnizO addr_map);
   wrapperG_var_lstoreG :> ghost_varG Σ lstore;
   wrapperG_var_lloc_mapG :> ghost_varG Σ lloc_map;
   wrapperG_var_bool :> ghost_varG Σ (leibnizO bool);
+}.
+
+Class wrapperGCtokG `{SI: indexT} Σ := WrapperGCtokG {
+  wrapperG_basics :> wrapperBasicsG Σ;
+  wrapperG_inG :> wrapperGCtokGpre Σ;
   wrapperG_γζ : gname;
   wrapperG_γθ : gname;
   wrapperG_γχ : gname;
@@ -51,7 +55,7 @@ Definition GC (θ : addr_map) : iProp Σ :=
   ∗ "GCroots" ∷ ghost_var wrapperG_γroots_set (1/2) roots_s
   ∗ "GCinit" ∷ ghost_var wrapperG_γat_init (1/2) false
   ∗ "GCζvirt" ∷ lstore_own_auth ζvirt
-  ∗ "(GCσMLv & GCσdom)" ∷ state_interp (σMLvirt : language.language.state ML_lang)
+  ∗ "GCσMLv" ∷ state_interp (σMLvirt : language.language.state ML_lang)
   ∗ "GCχvirt" ∷ lloc_own_auth χvirt
   ∗ "GCχNone" ∷ ([∗ map] _↦ℓ ∈ pub_locs_in_lstore χvirt ζvirt, ℓ ↦M/)
   ∗ "GCrootsm" ∷ ghost_map_auth wrapperG_γroots_map 1 roots_m
