theories/c_lang/mlang_instantiation.v
@@ -4,10 +4,17 @@ From iris.algebra Require Export ofe.
 From iris.heap_lang Require Export locations.
 From iris.prelude Require Import options.
 From melocoton.mlanguage Require Export mlanguage.
-From melocoton.c_lang Require Export lang metatheory.
+From melocoton.c_interface Require Export resources.
+From melocoton.c_lang Require Export lang metatheory primitive_laws.
 From melocoton.c_lang Require Import lang_instantiation.
-From melocoton.lang_to_mlang Require Import lang.
+From melocoton.lang_to_mlang Require Import lang weakestpre.
+From melocoton.mlanguage Require Import weakestpre.
+
 
 Canonical Structure C_mlang := (lang_to_mlang C_lang).
 
-
+Global Instance C_mlang_linkable `{SI: indexT} `{Σ: gFunctors} `{!heapG_C Σ}
+: linkableG (lang_to_mlang C_lang) public_state_interp.
+Proof.
+  apply lang_to_mlang_linkableG.
+Defined.
